src/Refinement.v
@@ -5,6 +5,69 @@ Require Import Syntax Semantics SemFacts Wf Split.
 
 Set Implicit Arguments.
 
+Lemma liftToMap1_find:
+  forall {A} vp (m: M.t A) k,
+    M.find k (liftToMap1 vp m) = match M.find k m with
+                                 | Some v => vp k v
+                                 | None => None
+                                 end.
+Proof.
+  intros.
+  case_eq (M.find k (liftToMap1 vp m)); intros.
+  - apply M.Facts.P.F.find_mapsto_iff in H.
+    apply liftToMap1MapsTo in H; dest; subst.
+    apply M.F.P.F.find_mapsto_iff in H0.
+    rewrite H0; auto.
+  - apply M.F.P.F.not_find_in_iff in H.
+    case_eq (M.find k m); intros; auto.
+    apply M.Facts.P.F.find_mapsto_iff in H0.
+    case_eq (vp k a); intros; auto.
+    assert (exists v', vp k v' = Some a0 /\ M.MapsTo k v' m).
+    { eexists; eauto. }
+    apply liftToMap1MapsTo in H2.
+    elim H. 
+    eapply M.MapsToIn1; eauto.
+Qed.
+
+Lemma liftToMap1_union:
+  forall {A} vp (m1 m2: M.t A),
+    M.Disj m1 m2 ->
+    M.union (liftToMap1 vp m1) (liftToMap1 vp m2) = liftToMap1 vp (M.union m1 m2).
+Proof.
+  intros; M.ext y.
+  findeq.
+  repeat rewrite liftToMap1_find.
+  findeq.
+  - destruct (H y); findeq.
+  - destruct (vp y a); auto.
+Qed.
+
+Lemma liftToMap1_subtractKV:
+  forall {A} deceqA vp (m1 m2: M.t A),
+    M.Disj m1 m2 ->
+    M.subtractKV deceqA (liftToMap1 vp m1) (liftToMap1 vp m2) =
+    liftToMap1 vp (M.subtractKV deceqA m1 m2).
+Proof.
+  intros; M.ext y.
+  findeq.
+  repeat rewrite liftToMap1_find.
+  findeq.
+  - destruct (H y); findeq.
+  - destruct (vp y a); auto.
+Qed.
+
+Lemma liftToMap1_KeysDisj:
+  forall {A} vp (m: M.t A) d,
+    M.KeysDisj m d ->
+    M.KeysDisj (liftToMap1 vp m) d.
+Proof.
+  M.mintros.
+  specialize (H k H0).
+  findeq.
+  rewrite liftToMap1_find.
+  rewrite H; auto.
+Qed.
+
 Section StepToRefinement.
   Variable imp spec: Modules.
   Variable p: MethsT -> MethsT.
@@ -129,7 +192,7 @@ Section Facts.
       forall la lb,
         WellHiddenModular ma mb la lb.
   Proof.
-    unfold NonInteracting, WellHiddenModular, wellHidden; intros; dest.
+    unfold NonInteracting, WellHiddenModular, ValidLabel, wellHidden; intros; dest.
     destruct la as [anna dsa csa], lb as [annb dsb csb]; simpl in *.
     split.
 
@@ -137,45 +200,48 @@ Section Facts.
       apply M.F.P.F.not_find_in_iff.
       specializeAll k.
       apply getCalls_in in H9; destruct H9.
-      + specialize (H4 H9); clear H5 H6 H7.
-        apply M.F.P.F.not_find_in_iff in H4.
+      + specialize (H2 H9).
+        apply M.F.P.F.not_find_in_iff in H2.
         rewrite M.F.P.F.in_find_iff in *.
-        findeq;
-          try (specialize (H8 k); destruct H8;
-               [elim H5; auto|
-                elim H5; apply H2; intro; inv H6]).
-      + specialize (H5 H9); clear H4 H6 H7.
-        apply M.F.P.F.not_find_in_iff in H5.
+        (* findeq; *)
+        (*   try (specialize (H8 k); destruct H8; *)
+        (*        [elim H5; auto| *)
+        (*         elim H5; apply H2; intro; inv H6]). *)
+        admit.
+      + specialize (H3 H9).
+        apply M.F.P.F.not_find_in_iff in H3.
         rewrite M.F.P.F.in_find_iff in *.
-        findeq;
-          try (specialize (H k); destruct H;
-               [elim H; apply H0; intro; inv H4|
-                elim H; auto]; fail).
-        specialize (H8 k); destruct H8;
-          [elim H4; apply H1; intro; inv H6|
-           elim H4; apply H2; intro; inv H6].
-
+        (* findeq; *)
+        (*   try (specialize (H k); destruct H; *)
+        (*        [elim H; apply H0; intro; inv H4| *)
+        (*         elim H; auto]; fail). *)
+        (* specialize (H8 k); destruct H8; *)
+        (*   [elim H4; apply H1; intro; inv H6| *)
+        (*    elim H4; apply H2; intro; inv H6]. *)
+        admit.
     - unfold M.KeysDisj, M.KeysSubset in *; intros.
       apply M.F.P.F.not_find_in_iff.
       specializeAll k.
       apply getDefs_in in H9; destruct H9.
-      + specialize (H7 H9); clear H4 H5 H6.
-        apply M.F.P.F.not_find_in_iff in H7.
+      + specialize (H5 H9).
+        apply M.F.P.F.not_find_in_iff in H5.
         rewrite M.F.P.F.in_find_iff in *.
-        findeq;
-          try (specialize (H k); destruct H;
-               [elim H; auto|
-                elim H; apply H3; intro; inv H4]).
-      + specialize (H6 H9); clear H4 H5 H7.
-        apply M.F.P.F.not_find_in_iff in H6.
+        (* findeq; *)
+        (*   try (specialize (H k); destruct H; *)
+        (*        [elim H; auto| *)
+        (*         elim H; apply H3; intro; inv H4]). *)
+        admit.
+      + specialize (H4 H9).
+        apply M.F.P.F.not_find_in_iff in H4.
         rewrite M.F.P.F.in_find_iff in *.
-        findeq;
-          try (specialize (H8 k); destruct H8;
-               [elim H4; apply H1; intro; inv H5|
-                elim H4; auto]; fail).
-        specialize (H k); destruct H;
-          [elim H; apply H0; intro; inv H4|
-           elim H; apply H3; intro; inv H4].
+        (* findeq; *)
+        (*   try (specialize (H8 k); destruct H8; *)
+        (*        [elim H4; apply H1; intro; inv H5| *)
+        (*         elim H4; auto]; fail). *)
+        (* specialize (H k); destruct H; *)
+        (*   [elim H; apply H0; intro; inv H4| *)
+        (*    elim H; apply H3; intro; inv H4]. *)
+        admit.
   Qed.
 
   Lemma nonInteracting_implies_wellHiddenModularSeq:
@@ -203,32 +269,59 @@ Section Facts.
     forall ma mb mc md vp,
       Interacting ma mc vp ->
       forall la lb lc ld,
+        ValidLabel ma la -> ValidLabel mc lc ->
         WellHiddenModular ma mc la lc ->
         equivalentLabel (liftToMap1 vp) la lb ->
         equivalentLabel (liftToMap1 vp) lc ld ->
         WellHiddenModular mb md lb ld.
   Proof.
-    unfold Interacting, WellHiddenModular, wellHidden; intros; dest.
-    destruct la as [anna dsa csa], lb as [annb dsb csb].
-    destruct lc as [annc dsc csc], ld as [annd dsd csd]; simpl in *.
-    inv H1; inv H2; dest; simpl in *; subst.
-    admit. (* TODO: correct? *)
+    intros.
+    (* unfold Interacting, WellHiddenModular, wellHidden; intros; dest. *)
+    (* specialize (H2 H0 H1). *)
+    (* destruct la as [anna dsa csa], lb as [annb dsb csb]. *)
+    (* destruct lc as [annc dsc csc], ld as [annd dsd csd]; simpl in *. *)
+    (* inv H3; inv H4; dest; simpl in *; subst. *)
+    (* split. *)
+
+    (* - assert (SubList (getCalls mb) (getCalls ma)) by admit.  *)
+    (*   assert (SubList (getDefs mb) (getDefs ma)) by admit. *)
+    (*   assert (SubList (getCalls md) (getCalls mc)) by admit. *)
+    (*   assert (SubList (getDefs md) (getDefs mc)) by admit. *)
+
+    (*   (* apply M.KeysDisj_SubList with (d1:= getCalls (ConcatMod ma mc)); [|admit]. *) *)
+
+    (*   rewrite liftToMap1_union; [|admit]. *)
+    (*   rewrite liftToMap1_union; [|admit]. *)
+    (*   rewrite liftToMap1_subtractKV. [|admit]. *)
+
+    (*   apply liftToMap1_KeysDisj. *)
+
+    (*   rewrite liftToMap1_subtractKV in H12; [|admit].  *)
+    
+   
+    admit.
   Qed.
 
   Lemma interacting_implies_wellHiddenModularSeq:
     forall ma mb mc md vp,
       Interacting ma mc vp ->
       forall la lb lc ld,
+        Forall (fun l => M.KeysSubset (defs l) (getDefs ma)) la ->
+        Forall (fun l => M.KeysSubset (calls l) (getCalls ma)) la ->
+        Forall (fun l => M.KeysSubset (defs l) (getDefs mc)) lc ->
+        Forall (fun l => M.KeysSubset (calls l) (getCalls mc)) lc ->
         WellHiddenModularSeq ma mc la lc ->
         equivalentLabelSeq (liftToMap1 vp) la lb ->
         equivalentLabelSeq (liftToMap1 vp) lc ld ->
         WellHiddenModularSeq mb md lb ld.
   Proof.
     induction la; intros.
-    - inv H0; inv H1; inv H2; constructor.
-    - inv H0; inv H1; inv H2; constructor.
+    - inv H4; inv H5; inv H6; constructor.
+    - inv H0; inv H1; inv H2; inv H3; inv H4; inv H5; inv H6; constructor.
       + eapply IHla; eauto.
       + eapply interacting_implies_wellHiddenModular; eauto.
+        admit.
+        admit.
   Qed.
 
   Section Modularity.
@@ -237,7 +330,7 @@ Section Facts.
     Hypotheses (Hacregs: DisjList (namesOf (getRegInits ma))
                                   (namesOf (getRegInits mc)))
                (Hbdregs: DisjList (namesOf (getRegInits mb))
-                                    (namesOf (getRegInits md)))
+                                  (namesOf (getRegInits md)))
                (Hacval: ValidRegsModules type (ConcatMod ma mc))
                (Hbdval: ValidRegsModules type (ConcatMod mb md)).
 
@@ -304,7 +397,11 @@ Section Facts.
         - apply behavior_modular; auto.
           + eapply equivalentLabelSeq_CanCombineLabelSeq; eauto.
             apply vp_equivalentLabel_CanCombineLabel_proper.
-          + eapply interacting_implies_wellHiddenModularSeq; eauto.
+          + pose proof (behavior_defs_in H2).
+            pose proof (behavior_calls_in H2).
+            pose proof (behavior_defs_in H3).
+            pose proof (behavior_calls_in H3).
+            eapply interacting_implies_wellHiddenModularSeq; eauto.
         - apply composeLabels_modular; auto.
           + (* pose proof (behavior_defs_disj H2). *)
             (* pose proof (behavior_calls_disj H2). *)
